Slight refinement: in PCUIC, use a common tagged sum for all primitive types

erasure/theories/EAst.v
@@ -1,5 +1,6 @@
 (* Distributed under the terms of the MIT license. *)
 From MetaCoq.Template Require Export utils BasicAst Universes.
+From MetaCoq.PCUIC Require Import PCUICPrimitive.
 (** * Extracted terms
 
   These are the terms produced by extraction: compared to kernel terms,
@@ -37,8 +38,7 @@ Inductive term : Set :=
 | tProj      : projection -> term -> term
 | tFix       : mfixpoint term -> nat -> term
 | tCoFix     : mfixpoint term -> nat -> term
-| tInt       : uint63_model -> term
-| tFloat     : float64_model -> term.
+| tPrim      : prim_val term -> term.
 
 Fixpoint mkApps t us :=
   match us with
