pcuic/theories/PCUICPrimitive.v
@@ -1,13 +1,13 @@
 (* Distributed under the terms of the MIT license. *)
-From MetaCoq.Template Require Export utils Universes BasicAst Reflect
+From MetaCoq.Template Require Import utils Universes BasicAst Reflect
      Environment EnvironmentTyping.
 From Equations Require Import Equations.
 From Coq Require Import ssreflect.
 
 Variant prim_tag := 
   | primInt
-  | primFloat
-  | primArray.
+  | primFloat.
+  (* | primArray. *)
 Derive NoConfusion EqDec for prim_tag.
 
 (** We don't enforce the type of the array here*)
@@ -26,15 +26,15 @@ Inductive prim_model (term : Type) : prim_tag -> Type :=
 (* | primArrayModel (a : array_model term) : prim_model term primArray. *)
 Arguments primIntModel {term}.
 Arguments primFloatModel {term}.
-Arguments primArrayModel {term}.
+(* Arguments primArrayModel {term}. *)
 
 Derive Signature NoConfusion for prim_model.
 
-Definition prim_model_of term (p : prim_tag) : Type := 
+Definition prim_model_of (term : Type) (p : prim_tag) : Type := 
   match p with
   | primInt => uint63_model
   | primFloat => float64_model
-  | primArray => array_model term
+  (* | primArray => array_model term *)
   end.
 
 Definition prim_val term := ∑ t : prim_tag, prim_model term t.
@@ -45,7 +45,7 @@ Definition prim_model_val {term} (p : prim_val term) : prim_model_of term (prim_
   match prim_val_model p in prim_model _ t return prim_model_of term t with
   | primIntModel i => i
   | primFloatModel f => f
-  | primArrayModel a => a
+  (* | primArrayModel a => a *)
   end.
 
 Lemma exist_irrel_eq {A} (P : A -> bool) (x y : sig P) : proj1_sig x = proj1_sig y -> x = y.
@@ -84,11 +84,13 @@ Qed.
 (** Propositional UIP is needed below *)
 Set Equations With UIP.
 
-Instance prim_model_eqdec {term} (e : EqDec term) : forall p : prim_tag, EqDec (prim_model term p).
+Instance prim_model_eqdec {term} (*e : EqDec term*) : forall p : prim_tag, EqDec (prim_model term p).
 Proof. eqdec_proof. Qed.
 
-Instance prim_tag_model_eqdec {term} (e : EqDec term) : EqDec (prim_val term).
+Instance prim_tag_model_eqdec term : EqDec (prim_val term).
 Proof. eqdec_proof. Defined.
+
+Instance prim_val_reflect_eq term : ReflectEq (prim_val term) := EqDec_ReflectEq _.
 
 (** Printing *)
 
@@ -99,5 +101,5 @@ Definition string_of_prim {term} (soft : term -> string) (p : prim_val term) : s
   match p.π2 return string with
   | primIntModel f => "(int: " ^ string_of_Z (proj1_sig f) ^ ")"
   | primFloatModel f => "(float: " ^ string_of_float64_model f ^ ")"
-  | primArrayModel a => "(array:" ^ ")"
+  (* | primArrayModel a => "(array:" ^ ")" *)
   end.
