erasure/theories/EOptimizePropDiscr.v
@@ -66,8 +66,7 @@ Section optimize.
     | tVar _ => t
     | tConst _ => t
     | tConstruct _ _ => t
-    | tInt _ => t
-    | tFloat _ => t
+    | tPrim _ => t
     end.
 
   Lemma optimize_mkApps f l : optimize (mkApps f l) = mkApps (optimize f) (map optimize l).
