pcuic/theories/PCUICNameless.v
@@ -47,7 +47,7 @@ Fixpoint nameless (t : term) : bool :=
   | tCoFix mfix idx =>
     forallb (fun d => banon d.(dname)) mfix &&
     forallb (test_def nameless nameless) mfix
-  | tInt _ | tFloat _ => true
+  | tPrim _ => true
   end.
 
 Definition anonymize (b : binder_annot name) : binder_annot name :=  
@@ -77,8 +77,7 @@ Fixpoint nl (t : term) : term :=
   | tProj p c => tProj p (nl c)
   | tFix mfix idx => tFix (map (map_def_anon nl nl) mfix) idx
   | tCoFix mfix idx => tCoFix (map (map_def_anon nl nl) mfix) idx
-  | tInt n => tInt n
-  | tFloat f => tFloat f
+  | tPrim p => tPrim p
   end.
 
 Definition map_decl_anon f (d : context_decl) := {|
