pcuic/theories/PCUICReflect.v
@@ -34,8 +34,7 @@ Local Ltac term_dec_tac term_dec :=
          | i : string, i' : kername |- _ => fcase (string_dec i i')
          | n : name, n' : name |- _ => fcase (eq_dec n n')
          | n : aname, n' : aname |- _ => fcase (eq_dec n n')
-         | i : uint63_model, j : uint63_model |- _ => fcase (eq_dec i j)
-         | i : float64_model, j : float64_model |- _ => fcase (eq_dec i j)
+         | i : prim_val, j : prim_val |- _ => fcase (eq_dec i j)
          | i : inductive, i' : inductive |- _ => fcase (eq_dec i i')
          | x : inductive * nat, y : inductive * nat |- _ =>
            fcase (eq_dec x y)
