safechecker/theories/Extraction.v
@@ -31,6 +31,7 @@ Extract Constant Equations.Init.pr1 => "fst".
 Extract Constant Equations.Init.pr2 => "snd".
 Extraction Inline Equations.Init.pr1 Equations.Init.pr2.
 Extraction Inline Equations.Prop.Logic.transport Equations.Prop.Logic.transport_r MCEquality.transport.
+Extraction Inline Equations.Prop.Logic.True_rect_dep Equations.Prop.Logic.False_rect_dep.
 
 Extract Constant PCUICTyping.guard_checking => "{ fix_guard = (fun _ _ _ -> true); cofix_guard = (fun _ _ _ -> true) }".
 
