safechecker/theories/PCUICSafeConversion.v
@@ -4058,31 +4058,14 @@ Section Conversion.
   Qed.
 
   (* TODO move to PCUICNormal *)
-  Lemma whnf_mkApps_tInt_inv : 
-    forall (f : RedFlags.t) (Σ : global_env) (Γ : context) i (args : list term),
-      whnf f Σ Γ (mkApps (tInt i) args) -> args = [].
+  Lemma whnf_mkApps_tPrim_inv : 
+    forall (f : RedFlags.t) (Σ : global_env) (Γ : context) p (args : list term),
+      whnf f Σ Γ (mkApps (tPrim p) args) -> args = [].
   Proof.
     intros * wh.
     inversion wh; solve_discr.
     clear -X.
-    remember (mkApps (tInt i) args) eqn:teq.
-    exfalso.
-    revert teq.
-    induction X in args |- *; intros; solve_discr.
-    destruct args as [|? ? _] using MCList.rev_ind; [easy|].
-    rewrite <- mkApps_nested in teq.
-    cbn in teq. noconf teq.
-    eauto.
-  Qed.
-  
-  Lemma whnf_mkApps_tFloat_inv : 
-    forall (rf : RedFlags.t) (Σ : global_env) (Γ : context) f (args : list term),
-      whnf rf Σ Γ (mkApps (tFloat f) args) -> args = [].
-  Proof.
-    intros * wh.
-    inversion wh; solve_discr.
-    clear -X.
-    remember (mkApps (tFloat f) args) eqn:teq.
+    remember (mkApps (tPrim p) args) eqn:teq.
     exfalso.
     revert teq.
     induction X in args |- *; intros; solve_discr.
@@ -4150,10 +4133,7 @@ Section Conversion.
     - constructor; eexists _, (decompose_stack π).1.
       split; [constructor; eauto with pcuic|].
       eauto with pcuic.
-    - apply whnf_mkApps_tInt_inv in wh as ->.
-      constructor; eexists _, [].
-      eauto using whnf_red with pcuic.
-    - apply whnf_mkApps_tFloat_inv in wh as ->.
+    - apply whnf_mkApps_tPrim_inv in wh as ->.
       constructor; eexists _, [].
       eauto using whnf_red with pcuic.
     - constructor; eexists _, (decompose_stack π).1.
@@ -4539,7 +4519,6 @@ Section Conversion.
       apply inversion_Sort in h2 as (_&h2&_); auto.
       apply inversion_Sort in h1 as (_&h1&_); auto.      
       eapply conv_pb_relb_complete in H0; eauto.
-    - now rewrite eq_dec_to_bool_refl in noteq.
     - now rewrite eq_dec_to_bool_refl in noteq.
   Qed.
   
